cleanup

Test/civl/samples/BroadcastConsensus.bpl
@@ -1,7 +1,7 @@
 // RUN: %parallel-boogie "%s" > "%t"
 // RUN: %diff "%s.expect" "%t"
 
-const MultisetEmpty:[val]int;
+const MultisetEmpty: [val]int;
 axiom MultisetEmpty == MapConst(0);
 
 function {:inline} MultisetSingleton(v:val) : [val]int
@@ -34,65 +34,86 @@ function {:inline} IsPid(i:int) : bool { 1 <= i && i <= n }
 
 ////////////////////////////////////////////////////////////////////////////////
 
-var {:layer 0,1} CH_low:[pid][val]int;
-var {:layer 1,2} CH:[val]int;
-var {:layer 0,2} {:linear} usedPermissions: Set Permission;
-var {:layer 0,2} value:[pid]val;
-var {:layer 0,2} decision:[pid]val;
+/*
+This is a two-layered proof of broadcast consensus.
+In the first layer, the Broadcast and Collect yield procedures performed by each process are
+converted into BROADCAST and COLLECT atomic actions, respectively.
+In the second layer, the body of Main comprising the broadcast loop followed by the collect
+loop are summarized.
+This summarization is enabled by a precondition on COLLECT that holds only after the
+broadcast loop is finished.
+This precondition is used to show that COLLECT is a left mover.
+*/
 
-function max(CH:[val]int) : val;
-function card(CH:[val]int) : int;
+// processes deposit Broadcast and Collect permissions in this global
+// variable once they are finished with the respective operations
+var {:layer 0,2} {:linear} usedPermissions: Set Permission;
+
+// array of values in the processes
+// each process broadcasts its value to all other processes
+var {:layer 0,2} value: [pid]val;
+
+// input channels for each process
+// each channel is modeled as a multiset
+var {:layer 0,1} channels: [pid][val]int;
+
+// processes store their consensus decision in this array
+// goal of verification is to prove that all values in decision are identical at the end
+var {:layer 0,2} decision: [pid]val;
+
+// multiset of values in the value array
+// abstraction of channels in program at layer 2
+var {:layer 1,2} values: [val]int;
+
+function max(values:[val]int) : val;
+function card(values:[val]int) : int;
 
 axiom card(MultisetEmpty) == 0;
-axiom (forall CH:[val]int, v:val, x:int :: card(CH[v := x]) == card(CH) + x - CH[v]);
+axiom (forall values:[val]int, v:val, x:int :: card(values[v := x]) == card(values) + x - values[v]);
 axiom (forall m:[val]int, m':[val]int :: MultisetSubsetEq(m, m') && card(m) == card(m') ==> m == m');
 
 axiom (forall v:val :: max(MultisetSingleton(v)) == v);
-axiom (forall CH:[val]int, v:val, x:int :: x > 0 ==> max(CH[v := x]) == (if v > max(CH) then v else max(CH)));
+axiom (forall values:[val]int, v:val, x:int :: x > 0 ==> max(values[v := x]) == (if v > max(values) then v else max(values)));
 
 function value_card(v:val, value:[pid]val, j:pid) : int
 {
   if j < 1 then
     0
+  else if value[j] == v then
+    value_card(v, value, j-1) + 1
   else
-    if value[j] == v then
-      value_card(v, value, j-1) + 1
-    else
-      value_card(v, value, j-1)
+    value_card(v, value, j-1)
 }
 
 ////////////////////////////////////////////////////////////////////////////////
 
-invariant {:layer 2} YieldCollect();
-preserves CH == (lambda v:val :: value_card(v, value, n));
-preserves card(CH) == n;
-preserves MultisetSubsetEq(MultisetEmpty, CH);
-preserves (forall q: Permission:: q is Broadcast && IsPid(q->i) ==> Set_Contains(usedPermissions, q));
-
-yield invariant {:layer 1} YieldInv();
-preserves Inv(CH_low, CH);
-
-function {:inline} Inv(CH_low:[pid][val]int, CH:[val]int) : bool
-{
-  (forall i:pid :: MultisetSubsetEq(MultisetEmpty, CH_low[i]) && MultisetSubsetEq(CH_low[i], CH))
-}
-
 yield invariant {:layer 1} YieldInit#1({:linear} ps: Set Permission);
 preserves ps->val == (lambda {:pool "A"} p: Permission ::IsPid(p->i));
-preserves (forall ii:pid :: CH_low[ii] == MultisetEmpty);
-preserves CH == MultisetEmpty;
+preserves (forall ii:pid :: channels[ii] == MultisetEmpty);
+preserves values == MultisetEmpty;
 preserves usedPermissions == Set_Empty();
 
 yield invariant {:layer 2} YieldInit#2({:linear} ps: Set Permission);
 preserves ps->val == (lambda {:pool "A"} p: Permission ::IsPid(p->i));
-preserves CH == MultisetEmpty;
+preserves values == MultisetEmpty;
 preserves usedPermissions == Set_Empty();
+
+yield invariant {:layer 1} YieldCollect();
+preserves (forall i:pid :: MultisetSubsetEq(MultisetEmpty, channels[i]) && MultisetSubsetEq(channels[i], values));
+
+invariant {:layer 2} CollectPre();
+preserves values == (lambda v:val :: value_card(v, value, n));
+preserves card(values) == n;
+preserves MultisetSubsetEq(MultisetEmpty, values);
+preserves (forall q: Permission:: q is Broadcast && IsPid(q->i) ==> Set_Contains(usedPermissions, q));
+
+////////////////////////////////////////////////////////////////////////////////
 
 yield left procedure {:layer 2} Main({:linear_in} ps: Set Permission)
 requires call YieldInit#1(ps);
 requires call YieldInit#2(ps);
-ensures {:layer 2} (forall j: pid:: 1 <= j && j <= n ==> decision[j] == max((lambda v: val:: value_card(v, value, n))));
-modifies CH, usedPermissions, decision;
+ensures {:layer 2} (forall j: pid:: IsPid(j) ==> decision[j] == max((lambda v: val:: value_card(v, value, n))));
+modifies values, usedPermissions, decision;
 {
   var i: pid;
   var {:linear} s: One Permission;
@@ -106,7 +127,7 @@ modifies CH, usedPermissions, decision;
   while (i <= n)
   invariant {:layer 1,2} 1 <= i && i <= n + 1;
   invariant {:layer 1,2} psb->val == (lambda p: Permission:: p is Broadcast && i <= p->i && p->i <= n);
-  invariant {:layer 2} MultisetSubsetEq(MultisetEmpty, CH) && CH == (lambda v: val:: value_card(v, value, i-1)) && card(CH) == i-1;
+  invariant {:layer 2} MultisetSubsetEq(MultisetEmpty, values) && values == (lambda v: val:: value_card(v, value, i-1)) && card(values) == i-1;
   invariant {:layer 2} Set((lambda p: Permission:: p is Broadcast && IsPid(p->i))) == Set_Union(usedPermissions, psb);
   {
     call s := One_Get(psb, Broadcast(i));
@@ -114,14 +135,14 @@ modifies CH, usedPermissions, decision;
     i := i + 1;
   }
 
-  assert {:layer 2} MultisetSubsetEq(MultisetEmpty, CH) && CH == (lambda v: val:: value_card(v, value, n)) && card(CH) == n;
+  assert {:layer 2} MultisetSubsetEq(MultisetEmpty, values) && values == (lambda v: val:: value_card(v, value, n)) && card(values) == n;
 
   i := 1;
   while (i <= n)
   invariant {:layer 1,2} 1 <= i && i <= n + 1;
   invariant {:layer 1,2} psc->val == (lambda p: Permission:: p is Collect && i <= p->i && p->i <= n);
   invariant {:layer 2} (forall q: Permission:: q is Broadcast && IsPid(q->i) ==> Set_Contains(usedPermissions, q));
-  invariant {:layer 2} (forall j: pid:: 1 <= j && j < i ==> decision[j] == max(CH));
+  invariant {:layer 2} (forall j: pid:: 1 <= j && j < i ==> decision[j] == max(values));
   {
     call r := One_Get(psc, Collect(i));
     async call {:sync} Collect(r, i);
@@ -130,11 +151,10 @@ modifies CH, usedPermissions, decision;
 }
 
 left action {:layer 2} BROADCAST({:linear_in} p: One Permission, i:pid)
-modifies CH;
 {
   assert IsPid(i) && p->val == Broadcast(i);
   assume {:add_to_pool "A", Broadcast(i)} true;
-  CH := CH[value[i] := CH[value[i]] + 1];
+  values := values[value[i] := values[value[i]] + 1];
   call One_Put(usedPermissions, p);
 }
 
@@ -144,47 +164,47 @@ requires {:layer 1} IsPid(i) && p->val == Broadcast(i);
 {
   var j: pid;
   var v: val;
-  var {:layer 1} old_CH_low: [pid][val]int;
+  var {:layer 1} old_channels: [pid][val]int;
 
-  call {:layer 1} old_CH_low := Copy(CH_low);
+  call {:layer 1} old_channels := Copy(channels);
   call v := get_value(i);
   j := 1;
   while (j <= n)
   invariant {:layer 1} 1 <= j && j <= n+1;
-  invariant {:layer 1} CH_low == (lambda jj: pid :: (if IsPid(jj) && jj < j then MultisetPlus(old_CH_low[jj], MultisetSingleton(value[p->val->i])) else old_CH_low[jj]));
+  invariant {:layer 1} channels == 
+    (lambda jj: pid :: (if IsPid(jj) && jj < j then MultisetPlus(old_channels[jj], MultisetSingleton(value[p->val->i])) else old_channels[jj]));
   {
     call send(v, j);
     j := j + 1;
   }
-  call {:layer 1} CH :=  Copy(CH[value[i] := CH[value[i]] + 1]);
+  call {:layer 1} values :=  Copy(values[value[i] := values[value[i]] + 1]);
   call release_permission(p);
 }
 
 left action {:layer 2} COLLECT({:linear_in} p: One Permission, i:pid)
-modifies decision;
-requires call YieldCollect();
+requires call CollectPre();
 {
   var received_values:[val]int;
   assert IsPid(i) && p->val == Collect(i);
   assume card(received_values) == n;
   assume MultisetSubsetEq(MultisetEmpty, received_values);
-  assume MultisetSubsetEq(received_values, CH);
+  assume MultisetSubsetEq(received_values, values);
   decision[i] := max(received_values);
   call One_Put(usedPermissions, p);
 }
 
 yield procedure {:layer 1} Collect({:linear_in} p: One Permission, i:pid)
 refines COLLECT;
-requires call YieldInv();
+requires call YieldCollect();
 requires {:layer 1} IsPid(i) && p->val == Collect(i);
 {
   var j: pid;
   var d: val;
   var v: val;
   var {:layer 1} received_values: [val]int;
-  var {:layer 1} old_CH_low: [pid][val]int;
+  var {:layer 1} old_channels: [pid][val]int;
 
-  call {:layer 1} old_CH_low := Copy(CH_low);
+  call {:layer 1} old_channels := Copy(channels);
   call d := receive(i);
   received_values := MultisetSingleton(d);
   j := 2;
@@ -192,8 +212,8 @@ requires {:layer 1} IsPid(i) && p->val == Collect(i);
   invariant {:layer 1} 2 <= j && j <= n + 1;
   invariant {:layer 1} card(received_values) == j - 1;
   invariant {:layer 1} MultisetSubsetEq(MultisetEmpty, received_values);
-  invariant {:layer 1} MultisetSubsetEq(received_values, old_CH_low[i]);
-  invariant {:layer 1} CH_low == old_CH_low[i := MapSub(old_CH_low[i], received_values)];
+  invariant {:layer 1} MultisetSubsetEq(received_values, old_channels[i]);
+  invariant {:layer 1} channels == old_channels[i := MapSub(old_channels[i], received_values)];
   invariant {:layer 1} d == max(received_values);
   {
     call v := receive(i);
@@ -206,43 +226,28 @@ requires {:layer 1} IsPid(i) && p->val == Collect(i);
 
 ////////////////////////////////////////////////////////////////////////////////
 
-both action {:layer 1} GET_VALUE(i:pid) returns (v:val)
-{
+yield procedure {:layer 0} get_value(i:pid) returns (v:val);
+refines both action {:layer 1} _ {
   v := value[i];
 }
 
-both action {:layer 1} SET_DECISION({:linear_in} p: One Permission, d:val)
-modifies decision, usedPermissions;
-{
+yield procedure {:layer 0} set_decision({:linear_in} p: One Permission, d:val);
+refines both action {:layer 1} _ {
   assert p->val is Collect;
   decision[p->val->i] := d;
   call One_Put(usedPermissions, p);
 }
 
-left action {:layer 1} SEND(v:val, i:pid)
-modifies CH_low;
-{
-  CH_low[i][v] := CH_low[i][v] + 1;
-}
-
-right action {:layer 1} RECEIVE(i:pid) returns (v:val)
-modifies CH_low;
-{
-  assume CH_low[i][v] > 0;
-  CH_low[i][v] := CH_low[i][v] - 1;
-}
-
-yield procedure {:layer 0} get_value(i:pid) returns (v:val);
-refines GET_VALUE;
-
-yield procedure {:layer 0} set_decision({:linear_in} p: One Permission, d:val);
-refines SET_DECISION;
-
 yield procedure {:layer 0} send(v:val, i:pid);
-refines SEND;
+refines left action {:layer 1} _ {
+  channels[i][v] := channels[i][v] + 1;
+}
 
 yield procedure {:layer 0} receive(i:pid) returns (v:val);
-refines RECEIVE;
+refines right action {:layer 1} _ {
+  assume channels[i][v] > 0;
+  channels[i][v] := channels[i][v] - 1;
+}
 
 yield procedure {:layer 0} release_permission({:linear_in} p: One Permission);
 refines both action {:layer 1} _ {
